

MIT Integration Bee: 2026 Final

Question 1

$$\lim_{n \rightarrow \infty} \int_0^1 \left(\sum_{k=1}^n \frac{1}{nx^2 + kx + n} \right) dx. \quad (1.1)$$

Solution The summation can be converted into a **Riemann sum**, which can be further recognized as an integral

$$\lim_{n \rightarrow \infty} \frac{1}{n} \sum_{k=1}^n \frac{1}{x^2 + \frac{k}{n}x + 1} = \int_0^1 \frac{dt}{x^2 + tx + 1} = \frac{\ln(x^2 + x + 1) - \ln(x^2 + 1)}{x}. \quad (1.2)$$

For the second term, we have (see [2024 Quarterfinal #2: Question 2](#))

$$I_2 = \int_0^1 \frac{\ln(1 + x^2)}{x} dx = \sum_{n=1}^{\infty} \frac{(-1)^{n-1}}{n} \int_0^1 x^{2n-1} dx = \sum_{n=1}^{\infty} \frac{(-1)^{n-1}}{2n^2} = \frac{\pi^2}{24}. \quad (1.3)$$

The infinite sum is from the **Basel problem** (see [2024 Final: Question 2](#)). For the first term, we can write it as

$$I_1 = \int_0^1 \frac{\ln(1 + x + x^2)}{x} dx = \int_0^1 \frac{\ln(1 - \omega x)}{x} dx + \int_0^1 \frac{\ln(1 - \omega^2 x)}{x} dx, \quad (1.4)$$

where $\omega = e^{2\pi i/3}$ is the **root of unity**. Similarly, based on the following result

$$\int_0^1 \frac{\ln(1 - \alpha x)}{x} dx = - \sum_{n=1}^{\infty} \frac{\alpha^n}{n} \int_0^1 x^{n-1} dx = - \frac{\alpha^n}{n^2}, \quad (1.5)$$

we have

$$I_1 = - \sum_{n=1}^{\infty} \frac{\omega^n + \omega^{2n}}{n^2} = -2 \sum_{n=1}^{\infty} \frac{\cos n\theta}{n^2}, \quad \text{with } \theta = \frac{2\pi}{3}. \quad (1.6)$$

Using the following **Fourier series**

$$(x - \pi)^2 = \frac{\pi^2}{3} + 4 \sum_{n=1}^{\infty} \frac{\cos nx}{n^2}, \quad x \in [0, \pi], \quad (1.7)$$

we can obtain

$$F(\theta) = \sum_{n=1}^{\infty} \frac{\cos n\theta}{n^2} = \frac{\pi^2}{6} - \frac{\pi\theta}{2} + \frac{\theta^2}{4}, \quad \theta \in [0, \pi]. \quad (1.8)$$

Finally, the original problem is solved as

$$I = I_1 - I_2 = -2F\left(\frac{2\pi}{3}\right) - \frac{\pi^2}{24} = \frac{\pi^2}{9} - \frac{\pi^2}{24} = \frac{5\pi^2}{72}. \quad (1.9)$$

Question 2

$$\int \frac{dx}{(x-1)\sqrt[4]{x^3+x}} \quad (2.1)$$

Solution Inspired by the **Euler substitution**, we use the following **change of variable**

$$t = \frac{\sqrt[4]{x^3+x}}{x+1}, \quad \frac{dt}{t} = \left[\frac{3x^2+1}{4x(x^2+1)} - \frac{1}{x+1} \right] dx = -\frac{(x-1)^3}{4x(x+1)(x^2+1)} dx. \quad (2.2)$$

We also obtain

$$x^3+x = t^4(x+1)^4, \quad \left(\frac{x-1}{x+1} \right)^4 = 1 - \frac{8(x^3+x)}{(x+1)^4} = 1 - 8t^4. \quad (2.3)$$

The integral now becomes

$$\begin{aligned} I &= - \int \frac{4(x^3+x)}{t^2(x-1)^4} dt = -4 \int t^2 \left(\frac{x+1}{x-1} \right)^4 dt = -4 \int \frac{t^2}{1-8t^4} dt \\ &= \frac{1}{\sqrt{2}} \left(\int \frac{dt}{2\sqrt{2}t^2+1} + \int \frac{dt}{2\sqrt{2}t^2-1} \right). \end{aligned} \quad (2.4)$$

With the following results

$$\int \frac{dt}{1+at^2} = \frac{1}{\sqrt{a}} \arctan(\sqrt{a}t) + C, \quad \int \frac{dt}{1-at^2} = \frac{1}{\sqrt{a}} \operatorname{arctanh}(\sqrt{a}t) + C, \quad (2.5)$$

the original problem is solved as

$$I = \frac{1}{2\sqrt[4]{2}} \left[\arctan \left(\frac{\sqrt[4]{8x^3+8x}}{x+1} \right) - \operatorname{arctanh} \left(\frac{\sqrt[4]{8x^3+8x}}{x+1} \right) \right] + C. \quad (2.6)$$

Question 3

$$\lim_{n \rightarrow \infty} \int_0^{2026} \underbrace{\log_{\sqrt{2}} \left(x + \log_{\sqrt{2}} \left(x + \cdots + \log_{\sqrt{2}} (x + 2026) \right) \right)}_{n \text{ logs}} dx \quad (3.1)$$

Solution Define the following function series

$$a_0(x) = 2026, \quad a_1(x) = \log_{\sqrt{2}}(x + a_0), \quad a_k(x) = \log_{\sqrt{2}}(x + a_{k-1}), \quad k \in \mathbb{N}^*. \quad (3.2)$$

As $k \rightarrow \infty$, denote $a_k(x) \rightarrow f(x)$ and we have

$$y = f(x) = \log_{\sqrt{2}}(x + f(x)), \quad x = t(y) = 2^{y/2} - y. \quad (3.3)$$

It can be shown that the series converges within the interval. Note that

$$t'(y) = 2^{y/2-1} \ln 2 - 1 > 0, \quad \forall y \geq 4; \quad t(4) = 0, \quad t(22) = 2026. \quad (3.4)$$

Therefore, using **integration by parts**, the integral is evaluated as

$$\begin{aligned} I &= \int_0^{2026} f(x) dx = [x f(x)]_0^{2026} - \int_4^{22} t(y) dy \\ &= 2026 \times 22 - \left[\frac{2^{y/2+1}}{\ln 2} - \frac{1}{2} y^2 \right]_4^{22} = 44806 - \frac{4088}{\ln 2}. \end{aligned} \quad (3.5)$$

Question 4

$$\int_0^{1/4} \left(\left[\sqrt[4]{\frac{1}{x} - 4} \right]^2 + \left[\sqrt[4]{\frac{1}{x} - 4} \right] \right) dx \quad (4.1)$$

Solution Note that

$$\left[\sqrt[4]{\frac{1}{x} - 4} \right] = k, \quad \text{when} \quad \frac{1}{(k+1)^4 + 4} < x \leq \frac{1}{k^4 + 4}. \quad (4.2)$$

The integral becomes the infinite sum

$$I = \sum_{k=0}^{\infty} k(k+1) \left[\frac{1}{k^4 + 4} - \frac{1}{(k+1)^4 + 4} \right] = \sum_{k=0}^{\infty} a_k (b_k - b_{k+1}), \quad (4.3)$$

where the two series $\{a_k\}$ and $\{b_k\}$ are defined as

$$a_k = k(k+1), \quad b_k = \frac{1}{k^4 + 4} \quad k \in \mathbb{N}. \quad (4.4)$$

Summation by parts leads to

$$I = a_0 b_0 + \sum_{k=1}^{\infty} (a_k - a_{k-1}) b_k = \sum_{k=1}^{\infty} \frac{2k}{k^4 + 4}. \quad (4.5)$$

This can be transformed into a **telescoping series** as

$$\frac{4k}{k^4 + 4} = \frac{1}{(k-1)^2 + 1} - \frac{1}{(k+1)^2 + 1}. \quad (4.6)$$

Therefore, the final result is obtained as

$$I = \frac{1}{2} \left(1 + \frac{1}{2} \right) = \frac{3}{4}. \quad (4.7)$$

Question 5

$$\int_{-\infty}^{+\infty} \left(\left(\frac{1}{x-2} + \frac{3}{x-4} + \frac{5}{x-6} \right)^{-2} + 1 \right)^{-1} dx \quad (5.1)$$

Solution Denote the partial fraction as $f(x)$, and then we have

$$I = \int_{-\infty}^{+\infty} \frac{f^2(x)}{1 + f^2(x)} dx, \quad f(x) = \frac{1}{x-2} + \frac{3}{x-4} + \frac{5}{x-6} = \sum_{j=1}^3 \frac{a_j}{x-m_j}. \quad (5.2)$$

Consider the following rational function in the complex plane

$$R(z) = \frac{f(z)}{1 + if(z)} = \frac{f(z) - if^2(z)}{1 + f^2(z)}. \quad (5.3)$$

First, the poles of $R(z)$ are all in the lower half-plane. This is because with $z = x + iy$, we have

$$1 + if(z) = 0 \quad \Leftrightarrow \quad f(z) = \sum_{j=1}^3 \frac{(x-m_j) a_j - iya_j}{(x-m_j)^2 + y^2} = i. \quad (5.4)$$

To satisfy this equation, we require $y < 0$ in the lower half-plane. From the **residue theorem**, the integral over a contour in the upper half-plane is zero for the rational function. As $z \rightarrow \infty$, we have

$$f(z) \rightarrow \frac{9}{z} + O\left(\frac{1}{z^2}\right), \quad R(z) \rightarrow \frac{9}{z} + O\left(\frac{1}{z^2}\right). \quad (5.5)$$

Therefore, we have

$$\lim_{R \rightarrow \infty} I_R = \lim_{R \rightarrow \infty} \int_{C_R} R(z) dz = 9\pi i. \quad (5.6)$$

This leads to

$$\int_{-\infty}^{+\infty} R(z) dz + \lim_{R \rightarrow \infty} I_R = 0, \quad \int_{-\infty}^{+\infty} R(z) dz = -9\pi i. \quad (5.7)$$

The original problem is thus evaluated as

$$I = -\text{Im} \int_{-\infty}^{+\infty} R(z) dz = 9\pi. \quad (5.8)$$